intermediate/Veritas.Intermediate.VerifyS.fsti
@@ -3,6 +3,7 @@ module Veritas.Intermediate.VerifyS
 open Veritas.Intermediate.Logs
 open Veritas.Intermediate.StoreS
 
+(* These are all independent of the 'verify' function; they should be safe to open *)
 open Veritas.BinTree
 open Veritas.Hash
 open Veritas.Key
@@ -11,9 +12,13 @@ open Veritas.MultiSetHashDomain
 open Veritas.Record
 open Veritas.SeqAux
 
+(* It's better not to open these modules to avoid naming conflicts *)
+module I = Veritas.Interleave
 module Spec = Veritas.Verifier
-module SC = Veritas.Intermediate.VerifySC
-module SCstore = Veritas.Intermediate.StoreSC
+module SpecVT = Veritas.Verifier.Thread
+module SpecVG = Veritas.Verifier.Global
+module SpecVTS = Veritas.Verifier.TSLog
+module SpecVC = Veritas.Verifier.Correctness
 
 (* Thread-local state
    id     : thread id
@@ -28,8 +33,8 @@ type vtls =
     id : thread_id ->
     st : vstore ->
     clock : timestamp ->
-    hadd : ms_hash_value -> // TODO: should be a multiset
-    hevict : ms_hash_value -> // TODO: should be a (multi?)set
+    hadd : ms_hash_value ->
+    hevict : ms_hash_value ->
     vtls
 
 let thread_id_of (vs:vtls {Valid? vs}): thread_id = 
@@ -38,8 +43,11 @@ let thread_id_of (vs:vtls {Valid? vs}): thread_id =
 let thread_store (vs: vtls {Valid? vs}): vstore =
   Valid?.st vs
 
+let thread_store_is_map (vs: vtls {Valid? vs}): bool =
+  let st = thread_store vs in st.is_map
+
 let thread_store_size (vs: vtls {Valid? vs}): nat =
-  let st = thread_store vs in Seq.length st
+  let st = thread_store vs in Seq.length st.data
 
 let update_thread_store (vs:vtls {Valid? vs}) (st:vstore) : vtls =
   match vs with
@@ -126,8 +134,8 @@ let vaddm (s:slot_id) (r:record) (s':slot_id) (vs: vtls {Valid? vs}): vtls =
             then (* k is a child of k' *)
               (* check hashes match and k was not evicted to blum *)
               if not (h2 = h && b2 = false) then Failed
-              (* check store does not contain k*)
-              else if child_in_store st s' d then Failed
+              (* check store does not contain k *)
+              else if in_store_bit st s' d then Failed
               else 
                 let st_upd = add_to_store st s k v Spec.MAdd in
                 let st_upd2 = update_in_store st_upd s' d true in
@@ -142,35 +150,24 @@ let vaddm (s:slot_id) (r:record) (s':slot_id) (vs: vtls {Valid? vs}): vtls =
               let mv = to_merkle_value v in
               let mv_upd = Spec.update_merkle_value mv d2 k2 h2 b2 in
               let v'_upd = Spec.update_merkle_value v' d k h false in
+              let od = other_dir d in
+              let od_bit = in_store_bit st s' od in // original in_store bit in the other direction
               let st_upd = update_value st s' (MVal v'_upd) in
               let st_upd2 = add_to_store st_upd s k (MVal mv_upd) Spec.MAdd in
               let st_upd3 = update_in_store st_upd2 s' d true in
-              let st_upd4 = update_in_store st_upd3 s d2 true in
-              update_thread_store vs st_upd4
+              let st_upd4 = update_in_store st_upd3 s' od od_bit in
+              let st_upd5 = update_in_store st_upd4 s d2 true in
+              update_thread_store vs st_upd5
 
 let has_instore_merkle_desc (st:vstore) (s:slot_id{store_contains st s}): bool = 
   let k = stored_key st s in
   if is_data_key k then false
   else 
-    // TODO: remove the assert with a better SMTPat for stored_value_matches_stored_key
-    let _ = assert (is_value_of k (stored_value st s)) in   
-    let v = to_merkle_value (stored_value st s) in
+    let _ = assert (is_value_of k (stored_value st s)) in
+    let v = to_merkle_value (stored_value_by_key st k) in
     let ld = desc_hash_dir v Left in
     let rd = desc_hash_dir v Right in
-    Desc? ld && l_child_in_store st s || 
-    Desc? rd && r_child_in_store st s
-
-let update_hash_and_blum_bit 
-      (st:vstore) 
-      (s:slot_id{store_contains st s /\ MVal? (stored_value st s)}) 
-      (d:bin_tree_dir{Desc? (desc_hash_dir (to_merkle_value (stored_value st s)) d)}) 
-      (h:hash_value)
-      (b:bool)
-  : vstore
-  = let mv = to_merkle_value (stored_value st s) in
-    let Desc k _ _ = desc_hash_dir mv d in
-    let mv' = Spec.update_merkle_value mv d k h b in
-    update_value st s (MVal mv')
+    Desc? ld && in_store_bit st s Left || Desc? rd && in_store_bit st s Right
 
 let vevictm (s:slot_id) (s':slot_id) (vs: vtls {Valid? vs}): vtls = 
   let st = thread_store vs in
@@ -183,7 +180,7 @@ let vevictm (s:slot_id) (s':slot_id) (vs: vtls {Valid? vs}): vtls =
     let v' = stored_value st s' in
     (* check k is a proper descendent of k' *)
     if not (is_proper_desc k k') then Failed
-    (* check k does not have a child in the store *)
+    (* check k does not have a (merkle) child in the store *)
     else if has_instore_merkle_desc st s then Failed
     else
       let d = desc_dir k k' in
@@ -197,7 +194,8 @@ let vevictm (s:slot_id) (s':slot_id) (vs: vtls {Valid? vs}): vtls =
       | Desc k2 h2 b2 -> 
           if k2 <> k then Failed
           else
-            let st_upd = update_hash_and_blum_bit st s' d h false in
+            let v'_upd = Spec.update_merkle_value v' d k h false in
+            let st_upd = update_value st s' (MVal v'_upd) in
             let st_upd2 = evict_from_store st_upd s in
             let st_upd3 = update_in_store st_upd2 s' d false in
             update_thread_store vs st_upd3
@@ -238,7 +236,7 @@ let vevictb (s:slot_id) (t:timestamp) (vs:vtls {Valid? vs}): vtls =
     else if not (ts_lt clock t) then Failed
     (* check s was added through blum *)  
     else if add_method_of st s <> Spec.BAdd then Failed
-    (* check k has no children n the store *)
+    (* check k has no (merkle) children n the store *)
     else if has_instore_merkle_desc st s then Failed  
     else 
       (* update evict hash *)
@@ -263,7 +261,7 @@ let vevictbm (s:slot_id) (s':slot_id) (t:timestamp) (vs:vtls {Valid? vs}): vtls 
     if not (is_proper_desc k k') then Failed
     (* check s was added through merkle *)
     else if add_method_of st s <> Spec.MAdd then Failed  
-    (* check k has no children in the store *)
+    (* check k has no (merkle) children in the store *)
     else if has_instore_merkle_desc st s then Failed  
     else
       // TODO: remove the assert with a better SMTPat for stored_value_matches_stored_key
@@ -276,9 +274,22 @@ let vevictbm (s:slot_id) (s':slot_id) (t:timestamp) (vs:vtls {Valid? vs}): vtls 
       | Desc k2 h2 b2 -> 
           if k2 <> k || b2 then Failed
           else
-            let st_upd = update_hash_and_blum_bit st s' d h2 true in
-            vevictb s t (update_thread_store vs st_upd)
-  
+            let v'_upd = Spec.update_merkle_value v' d k h2 true in
+            let st_upd = update_value st s' (MVal v'_upd) in
+            let st_upd2 = update_in_store st_upd s' d false in
+            vevictb s t (update_thread_store vs st_upd2)
+
+(* Relation between thread-local states *)
+(* either both states have Failed, or both are Valid with equal contents AND the
+   is_map flag in vs is true *)
+let vtls_rel (vs:vtls) (vs':Spec.vtls) : Type =
+  (Failed? vs /\ Spec.Failed? vs') \/
+  (Valid? vs /\ Spec.Valid? vs' /\
+   (let Valid id st clk ha he = vs in
+    let Spec.Valid id' st' clk' _ ha' he' = vs' in
+    st.is_map /\ store_rel st st' /\
+    id = id' /\ clk = clk' /\ ha = ha' /\ he = he'))
+
 let t_verify_step (vs:vtls) (e:logS_entry): vtls =
   match vs with
   | Failed -> Failed
@@ -292,16 +303,33 @@ let t_verify_step (vs:vtls) (e:logS_entry): vtls =
     | EvictB_S s t -> vevictb s t vs
     | EvictBM_S s s' t -> vevictbm s s' t vs
 
-(* Verify a (thread-local) log from a specified initial state *)
-let rec t_verify_aux (vs:vtls) (l:logS): Tot vtls
+(* convert slot-based log entry e to a key-based log entry, given verifier state vtls *)
+val logS_to_logK_entry (vs:vtls{Valid? vs}) (e:logS_entry) : option logK_entry
+
+let add_to_log (l:option logK) (vs:vtls) (e:logS_entry) : option logK =
+  if Some? l && Valid? vs && Some? (logS_to_logK_entry vs e)
+  then Some (append1 (Some?.v l) (Some?.v (logS_to_logK_entry vs e)))
+  else None
+
+(* Verify a log from a specified initial state; also returns the
+   corresponding log with keys *)
+let rec t_verify_aux (vs:vtls) (l:logS): Tot (vtls * option logK)
   (decreases (Seq.length l)) =
   let n = Seq.length l in
-  if n = 0 then vs
+  if n = 0 then (vs, Some Seq.empty)
   else
     let lp = prefix l (n - 1) in
-    let vsp = t_verify_aux vs lp in
+    let (vsp,lk) = t_verify_aux vs lp in
     let e = Seq.index l (n - 1) in
-    t_verify_step vsp e
+    let vs' = t_verify_step vsp e in
+    let lk' = add_to_log lk vsp e in
+    (vs', lk')
+
+val lemma_t_verify_aux_valid_implies_log_exists (vs:vtls) (l:logS)
+  : Lemma (requires (Valid? (fst (t_verify_aux vs l))))
+          (ensures (Some? (snd (t_verify_aux vs l))))
+          (decreases (Seq.length l))
+          [SMTPat (Some? (snd (t_verify_aux vs l)))]
 
 (* Initialize verifier state *)
 // TODO: what should the initial size be?
@@ -316,45 +344,79 @@ let init_thread_state (id:thread_id): vtls =
 
 (* Main thread-level verify function *)
 let t_verify (id:thread_id) (l:logS): vtls = 
-  t_verify_aux (init_thread_state id) l 
+  fst (t_verify_aux (init_thread_state id) l) 
 
-(* Relation between SC and S thread-local states *)
-let vtls_rel (vs:vtls) (vs':SC.vtls) : Type =
-  (Failed? vs /\ SC.Failed? vs') \/
-  (Valid? vs /\ SC.Valid? vs' /\
-   (let (Valid id st clk ha he) = vs in
-    let (SC.Valid id' st' clk' ha' he') = vs' in
-    // all fields are equal
-    equal_contents st st' /\ id = id' /\ clk = clk' /\ ha = ha' /\ he = he'))
+let logS_to_logK (id:thread_id) (l:logS{Valid? (t_verify id l)}) : logK =
+  Some?.v (snd (t_verify_aux (init_thread_state id) l))
 
 let init_thread_state_valid (id:thread_id)
   : Lemma (Valid? (init_thread_state id))
           [SMTPat (init_thread_state id)]
   = ()
 
-val lemma_init_thread_state_rel (id:thread_id)
-  : Lemma (vtls_rel (init_thread_state id) (SC.init_thread_state id))
+val lemma_init_thread_state_rel (id:thread_id) :
+  Lemma (vtls_rel (init_thread_state id) (Spec.init_thread_state id))
 
-val lemma_t_verify_simulates_SC (id:thread_id) (l:logS) 
-  : Lemma (vtls_rel (t_verify id l) (SC.t_verify id l))
+val lemma_t_verify_simulates_spec (id:thread_id) (l:logS) 
+  : Lemma (requires (Valid? (t_verify id l)))
+          (ensures (vtls_rel (t_verify id l) (Spec.t_verify id (logS_to_logK id l))))
 
-(* Global verification *)
+val lemma_logS_to_logK_to_state_op (id:thread_id) (l:logS{Valid? (t_verify id l)})
+  : Lemma (ensures (Seq.equal (to_state_op_logS l) 
+                              (Veritas.EAC.to_state_op_vlog (logS_to_logK id l))))
+           [SMTPat (Veritas.EAC.to_state_op_vlog (logS_to_logK id l))]
+
+(* Utilities for running a single verifier thread.
+   Follows the definitions in Veritas.Verifier.Thread. *)
+
 let verify (tl:thread_id_logS): vtls =
   t_verify (fst tl) (snd tl)
-
-let tl_verifiable (tl: thread_id_logS) = 
+  
+let tl_verifiable (tl: thread_id_logS): bool =
   Valid? (verify tl)
 
+let tl_verifiable_log = tl: thread_id_logS {tl_verifiable tl}
+
+val lemma_tl_verifiable_implies_prefix_verifiable
+  (tl:tl_verifiable_log) (i:nat{i <= tl_length tl}):
+  Lemma (ensures (tl_verifiable (tl_prefix tl i)))
+        [SMTPat (tl_prefix tl i)]
+
+let tl_clock (tl:tl_verifiable_log) (i:tl_idx tl): timestamp =
+  Valid?.clock (verify (tl_prefix tl (i + 1)))
+
+let tl_verify (tl:thread_id_logS) (i:tl_idx tl): vtls =
+  verify (tl_prefix tl (i + 1))
+
+let tl_logS_to_logK (tl:tl_verifiable_log{thread_store_is_map (verify tl)}) 
+  : SpecVT.verifiable_log
+  = lemma_t_verify_simulates_spec (fst tl) (snd tl);
+    (fst tl, logS_to_logK (fst tl) (snd tl))
+
+let lemma_tl_length (tl:tl_verifiable_log{thread_store_is_map (verify tl)})
+  : Lemma (ensures tl_length tl = SpecVT.length (tl_logS_to_logK tl))
+          [SMTPat (tl_length tl)]
+  = admit()
+
+// may be useful
+let lemma_tl_clock_simulates_spec (tl: tl_verifiable_log{thread_store_is_map (verify tl)}) (i:tl_idx tl)
+  : Lemma (tl_clock tl i = SpecVT.clock (tl_logS_to_logK tl) i)
+  = admit()
+
+(* Utilities for running all verifier threads and comparing aggregate add/evict hashes.
+   Follows the definitions in Veritas.Verifier.Global. *) 
+
 let gl_verifiable (gl: g_logS) = 
-  forall (tid:seq_index gl). Valid? (verify (thread_log gl tid))
+  forall (tid:seq_index gl). tl_verifiable (thread_log gl tid)
 
-let tl_verifiable_log = gl:g_logS{tl_verifiable gl}
+let gl_verifiable_log = gl:g_logS{gl_verifiable gl}
 
-val lemma_prefix_tl_verifiable (gl: tl_verifiable_log) (i:seq_index gl)
-  : Lemma (ensures tl_verifiable (prefix gl i))
-          [SMTPat (tl_verifiable (prefix gl i))]
+val lemma_gl_verifiable_implies_prefix_verifiable
+  (gl:gl_verifiable_log) (i:nat{i <= Seq.length gl}):
+  Lemma (ensures (gl_verifiable (prefix gl i)))
+        [SMTPat (prefix gl i)]
 
-let rec hadd_aux (gl: tl_verifiable_log)
+let rec hadd_aux (gl: gl_verifiable_log)
   : Tot (ms_hash_value)
     (decreases (Seq.length gl)) 
   = let p = Seq.length gl in
@@ -365,9 +427,9 @@ let rec hadd_aux (gl: tl_verifiable_log)
       let h2 = thread_hadd (verify (thread_log gl (p - 1))) in
       ms_hashfn_agg h1 h2
 
-let hadd (gl: tl_verifiable_log): ms_hash_value = hadd_aux gl
+let hadd (gl: gl_verifiable_log): ms_hash_value = hadd_aux gl
 
-let rec hevict_aux (gl: tl_verifiable_log)
+let rec hevict_aux (gl: gl_verifiable_log)
   : Tot (ms_hash_value)
     (decreases (Seq.length gl))
   = let p = Seq.length gl in
@@ -378,39 +440,87 @@ let rec hevict_aux (gl: tl_verifiable_log)
       let h2 = thread_hevict (verify (thread_log gl (p - 1))) in
       ms_hashfn_agg h1 h2
 
-let hevict (gl: tl_verifiable_log): ms_hash_value = hevict_aux gl
+let hevict (gl: gl_verifiable_log): ms_hash_value = hevict_aux gl
 
-let hash_verifiable (gl: verifiable_log): bool
-  = hadd gl = hevict gl
+let gl_hash_verifiable (gl: gl_verifiable_log): bool = 
+  hadd gl = hevict gl
 
-let hash_verifiable_log = gl:verifiable_log{hash_verifiable gl}
+let gl_hash_verifiable_log = gl:gl_verifiable_log{gl_hash_verifiable gl}
 
-let lemma_verifiable_simulates_SC (gl:verifiable_log)
-  : Lemma (ensures SC.verifiable gl)
-          [SMTPat (SC.verifiable gl)]
-  = let aux (tid:seq_index gl) : Lemma (SC.Valid? (SC.verify (thread_log gl tid)))
-      = lemma_t_verify_simulates_SC tid (Seq.index gl tid) in
+let gl_clock (gl:gl_verifiable_log) (i:I.sseq_index gl): timestamp = 
+  let (tid, idx) = i in  
+  let tl = thread_log gl tid in
+  tl_clock tl idx
+
+let gl_verify (gl:g_logS) (i:I.sseq_index gl): vtls =
+  let (tid, idx) = i in  
+  let tl = thread_log gl tid in
+  tl_verify tl idx
+
+let forall_is_map (gl:gl_verifiable_log)
+  = forall (tid:seq_index gl). thread_store_is_map (verify (thread_log gl tid))
+
+val forall_is_mapb (gl:gl_verifiable_log) : bool
+
+val lemma_forall_is_mapb (gl:gl_verifiable_log)
+  : Lemma (ensures (forall_is_map gl <==> forall_is_mapb gl))
+          [SMTPat (forall_is_mapb gl)]
+
+val glogS_to_logK (gl:gl_verifiable_log{forall_is_map gl}) 
+  : gl':SpecVG.verifiable_log{Seq.length gl = Seq.length gl'}
+
+val lemma_glogS_to_logK (gl:gl_verifiable_log{forall_is_map gl}) (id:seq_index gl)
+  : Lemma (ensures Seq.index (glogS_to_logK gl) id = logS_to_logK id (Seq.index gl id))
+          [SMTPat (Seq.index (glogS_to_logK gl) id)]
+
+val lemma_hadd_equal (gl:gl_verifiable_log{forall_is_map gl}) 
+  : Lemma (hadd gl = SpecVG.hadd (glogS_to_logK gl))
+
+val lemma_hevict_equal (gl:gl_verifiable_log{forall_is_map gl}) 
+  : Lemma (hevict gl = SpecVG.hevict (glogS_to_logK gl))
+
+let lemma_gl_hash_verifiable_simulates_spec (gl:gl_hash_verifiable_log{forall_is_map gl})
+  : Lemma (SpecVG.hash_verifiable (glogS_to_logK gl))
+  = lemma_hadd_equal gl;
+    lemma_hevict_equal gl
+
+let lemma_to_state_op_glogS (gl: gl_verifiable_log{forall_is_map gl})
+  : Lemma (ensures (Seq.equal (to_state_op_glogS gl) 
+                              (SpecVC.to_state_op_gvlog (glogS_to_logK gl))))
+  = let aux (i:seq_index gl) 
+      : Lemma (Seq.index (to_state_op_glogS gl) i = 
+              Seq.index (SpecVC.to_state_op_gvlog (glogS_to_logK gl)) i)
+      = () in
     Classical.forall_intro aux
 
-val hadd_values_equal (gl:verifiable_log) : Lemma (hadd gl = SC.hadd gl)
+(* Utilities for verifying the global, interleaved log shared among all threads.
+   Follows the definitions in Veritas.Verifier.TSLog. *) 
 
-val hevict_values_equal (gl:verifiable_log) : Lemma (hevict gl = SC.hevict gl)
+let il_verifiable (il: il_logS) = 
+  gl_verifiable (g_logS_of il)
 
-let lemma_hash_verifiable_simulates_SC (gl:hash_verifiable_log)
-  : Lemma (SC.hash_verifiable gl)
-  = hadd_values_equal gl;
-    hevict_values_equal gl
+let il_clock (il: il_logS{il_verifiable il}) (i: I.seq_index il): timestamp =
+  let gl = g_logS_of il in
+  let j = I.i2s_map il i in
+  gl_clock gl j
 
-(* Correctness *)
+(* state at thread j after processing log entry i (which modifies the state of j) *)
+let il_verify (il: il_logS) (i: I.seq_index il): vtls =
+  let gl = g_logS_of il in
+  let j = I.i2s_map il i in
+  gl_verify gl j
 
-let lemma_verifier_correct (gl: hash_verifiable_log { ~ (Veritas.State.seq_consistent (to_state_op_glogS gl))})
-  : Veritas.Verifier.EAC.hash_collision_gen
-  = let itsl = il_create gl in
-    // destruct on (is_eac itsl)
-    // in the true case
-    //   we should be able to prove that the S/SC vfun functions always produce related results;
-    //   so we can reuse SC.lemma_verifier_correct
-    // in the false case
-    //   we should be able to generate a hash collision; 
-    //   can we reuse Veritas.Verifier.EAC.lemma_non_eac_time_seq_implies_hash_collision?
-    admit()
+val clock_sorted (il: il_logS {il_verifiable il}): prop
+ 
+let its_log = il:il_logS{il_verifiable il /\ clock_sorted il}
+
+let il_hash_verifiable (itsl: its_log) = gl_hash_verifiable (g_logS_of itsl)
+
+let il_hash_verifiable_log = itsl:its_log {il_hash_verifiable itsl}
+
+val lemma_prefix_verifiable (itsl: its_log) (i:nat{i <= I.length itsl}):
+  Lemma (ensures (il_verifiable (I.prefix itsl i) /\ clock_sorted (I.prefix itsl i)))
+        [SMTPat (I.prefix itsl i)]
+
+val il_create (gl: gl_verifiable_log): (itsl:its_log{g_logS_of itsl == gl})
+
